filling in some good to have instances

src/computational_monads/simulation_semantics/oracle_compose.lean
@@ -23,8 +23,9 @@ namespace sim_oracle
 For example a random oracle is a uniform oracle composed with a cacheing oracle,
 i.e. one that caches previous responses and calls a uniform random oracle for any new queries.
 For type inference reasons we list the arguments in the opposite order of `function.comp`. -/
-def compose (so' : sim_oracle spec' spec'' S') (so : sim_oracle spec spec' S) : sim_oracle spec spec'' (S × S') :=
-λ i x, simulate so' (so i (x.1, x.2.1)) x.2.2 >>= λ u_s, return (u_s.1.1, u_s.1.2, u_s.2)
+def compose (so' : sim_oracle spec' spec'' S') (so : sim_oracle spec spec' S) :
+  sim_oracle spec spec'' (S × S') :=
+λ i x, (λ z : (_ × S) × S', (z.1.1, z.1.2, z.2)) <$> simulate so' (so i (x.1, x.2.1)) x.2.2
 
 -- We use `notation` over `infixl` to swap the arguments without invoking `function.comp`.
 notation so' `∘ₛₒ` so := so'.compose so
@@ -33,12 +34,12 @@ namespace oracle_compose
 
 variables (so : sim_oracle spec spec' S) (so' : sim_oracle spec' spec'' S')
 
-@[simp] lemma apply_eq (i : spec.ι) (z : spec.domain i × S × S') : (so' ∘ₛₒ so) i z =
-  simulate so' (so i (z.1, z.2.1)) z.2.2 >>= λ z', return (z'.1.1, z'.1.2, z'.2) := rfl
+@[simp] lemma apply_eq (i : spec.ι) (x : spec.domain i × S × S') : (so' ∘ₛₒ so) i x =
+  (λ z : (_ × S) × S', (z.1.1, z.1.2, z.2)) <$> simulate so' (so i (x.1, x.2.1)) x.2.2 := rfl
 
 instance is_tracking (so : sim_oracle spec spec S) (so' : sim_oracle spec spec S')
   [hso : so.is_tracking] [hso' : so'.is_tracking] : (so' ∘ₛₒ so).is_tracking :=
-⟨λ i t s, by rw [apply_eq, fst_map_bind_return, ← map_map_eq_map_comp _ prod.fst prod.fst,
+⟨λ i t s, by rw [apply_eq, map_map_eq_map_comp, ← map_map_eq_map_comp _ prod.fst prod.fst,
   ← simulate', is_tracking.simulate'_eq_self, is_tracking.fst_map_apply_eq_query]⟩
 
 end oracle_compose
