src/computational_monads/coercions/instances.lean
@@ -5,6 +5,7 @@ Authors: Devon Tuma
 -/
 import computational_monads.coercions.sub_spec
 import computational_monads.constructions.uniform_select
+import computational_monads.simulation_semantics.oracle_append
 
 /-!
 # Sub-Spec Instances for Common Sets of Oracles
@@ -39,11 +40,11 @@ This ordering is chosen to both give a generally applicable instance tree,
 and avoid an infinite typeclass search whether or not an instance exists.
 -/
 
-variables {α β γ : Type}
-
 namespace oracle_spec
 
 open oracle_comp
+
+variables {spec spec' spec'' : oracle_spec} {α β γ S S' : Type}
 
 section empty_spec
 
@@ -63,8 +64,7 @@ section coin_spec_unif_spec
 /-- Coerce a coin flip into a uniform random selection of a `bool`.
 Use uniform selection from the vector `[tt, ff]` to get constructiveness. -/
 @[priority std.priority.default+100]
-noncomputable instance is_sub_spec_coin_spec_unif_spec :
-  is_sub_spec coin_spec unif_spec :=
+noncomputable instance is_sub_spec_coin_spec_unif_spec : is_sub_spec coin_spec unif_spec :=
 { to_fun := λ i t, $ᵗ bool,
   to_fun_equiv := λ i t, symm ((query_dist_equiv_iff i t _).2
     (λ u u', by cases u; cases u'; simp [prob_output_uniform_select_fintype bool])) }
@@ -77,6 +77,8 @@ noncomputable instance is_sub_spec_coin_spec_unif_spec :
 
 end coin_spec_unif_spec
 
+section append_left
+
 /-- Coerce a computation to one with access to another oracle on the left,
 forwarding the old queries to the left side of the combined set of oracles. -/
 @[priority std.priority.default]
@@ -84,11 +86,27 @@ instance is_sub_spec_append_left (spec spec' : oracle_spec) : spec ⊂ₒ (spec'
 { to_fun := λ i t, @query (spec' ++ spec) (sum.inr i) t,
   to_fun_equiv := λ i t, trans (eval_dist_query (sum.inr i) t) (eval_dist_query i t).symm }
 
-@[simp] lemma is_sub_spec_append_left_apply {spec spec' : oracle_spec}
-  (i : spec.ι) (t : spec.domain i) : (oracle_spec.is_sub_spec_append_left spec spec').to_fun i t =
+@[simp] lemma is_sub_spec_append_left_apply (i : spec.ι) (t : spec.domain i) :
+  (oracle_spec.is_sub_spec_append_left spec spec').to_fun i t =
     @query (spec' ++ spec) (sum.inr i) t := rfl
 
--- TODO: eventually it would be good to add simp lemmas for the rest of these.
+variables (so : sim_oracle spec spec'' S) (so' : sim_oracle spec' spec'' S')
+
+@[simp] lemma simulate_coe_append_left (s : S × S') (oa : oracle_comp spec' α) :
+  simulate (so ++ₛₒ so') ↑oa s = (λ (x : α × S'), (x.1, s.1, x.2)) <$> simulate so' oa s.2 :=
+begin
+  induction oa using oracle_comp.induction_on' with α a i t α oa hoa generalizing s,
+  { simp only [coe_sub_spec_return, simulate_return, map_pure, prod.mk.eta] },
+  { simp [hoa, bind_assoc, oracle_comp.map_eq_bind_return_comp] }
+end
+
+@[simp] lemma simulate'_coe_append_left (s : S × S') (oa : oracle_comp spec' α) :
+  (simulate' (so ++ₛₒ so') ↑oa s) = simulate' so' oa s.2 :=
+by simp [simulate'.def]
+
+end append_left
+
+section append_right
 
 /-- Coerce a computation to one with access to another oracle on the right,
 forwarding the old queries to the left side of the combined set of oracles. -/
@@ -101,6 +119,24 @@ instance is_sub_spec_append_right (spec spec' : oracle_spec) : spec ⊂ₒ (spec
   (i : spec.ι) (t : spec.domain i) : (oracle_spec.is_sub_spec_append_right spec spec').to_fun i t =
     @query (spec ++ spec') (sum.inl i) t := rfl
 
+variables (so : sim_oracle spec spec'' S) (so' : sim_oracle spec' spec'' S')
+
+@[simp] lemma simulate_coe_append_right (s : S × S') (oa : oracle_comp spec α) :
+  simulate (so ++ₛₒ so') ↑oa s = (λ (x : α × S), (x.1, x.2, s.2)) <$> simulate so oa s.1 :=
+begin
+  induction oa using oracle_comp.induction_on' with α a i t α oa hoa generalizing s,
+  { simp only [coe_sub_spec_return, simulate_return, map_pure, prod.mk.eta] },
+  { simp [hoa, bind_assoc, oracle_comp.map_eq_bind_return_comp] }
+end
+
+@[simp] lemma simulate'_coe_append_right (s : S × S') (oa : oracle_comp spec α) :
+  (simulate' (so ++ₛₒ so') ↑oa s) = simulate' so oa s.1 :=
+by simp [simulate'.def]
+
+end append_right
+
+section append_left_of_is_subspec
+
 /-- Coerce an oracle and then append to the left. Already sort of exists,
   but the instance priorities don't work without explicitly having this. -/
 @[priority std.priority.default+10]
@@ -110,6 +146,10 @@ instance is_sub_spec_append_left_of_is_sub_spec
 { to_fun := λ i t, ↑(h.to_fun i t),
   to_fun_equiv := λ i t, (eval_dist_coe_sub_spec _ _ _).trans (is_sub_spec.to_fun_equiv _ _) }
 
+end append_left_of_is_subspec
+
+section append_right_of_is_subspec
+
 /-- Coerce an oracle and then append to the right. Already sort of exists,
   but the instance priorities don't work without explicitly having this. -/
 @[priority std.priority.default+11]
@@ -118,6 +158,10 @@ instance is_sub_spec_append_right_of_is_sub_spec
   [h : is_sub_spec sub_spec super_spec] : is_sub_spec sub_spec (super_spec ++ spec) :=
 { to_fun := λ i t, ↑(h.to_fun i t),
   to_fun_equiv := λ i t, (eval_dist_coe_sub_spec _ _ _).trans (is_sub_spec.to_fun_equiv _ _) }
+
+end append_right_of_is_subspec
+
+section left_side_append
 
 /-- Coerce the oracle on the right side of an existing set of appended oracles. -/
 @[priority std.priority.default+20]
@@ -134,6 +178,10 @@ instance is_sub_spec_left_side_append
   | (sum.inr i) := λ t, rfl
   end }
 
+end left_side_append
+
+section right_side_append
+
 /-- Coerce the oracle on the right side of an existing set of appended oracles. -/
 @[priority std.priority.default+21]
 instance is_sub_spec_right_side_append (spec sub_spec super_spec : oracle_spec)
@@ -147,6 +195,10 @@ instance is_sub_spec_right_side_append (spec sub_spec super_spec : oracle_spec)
   | (sum.inr i) := λ t, (eval_dist_coe_sub_spec _ _ (h.to_fun i t)).trans
       ((h.to_fun_equiv i t).trans (by exact rfl))
   end }
+
+end right_side_append
+
+section assoc
 
 /-- Coerce towards a standardized append ordering (matching the `infixl` declaration for `++`) -/
 @[priority std.priority.default+30]
@@ -163,6 +215,8 @@ instance is_sub_spec_assoc (spec spec' spec'' : oracle_spec) :
   | (sum.inr (sum.inr i)) := λ t, rfl
   end }
 
+end assoc
+
 end oracle_spec
 
 namespace oracle_spec
@@ -171,10 +225,8 @@ open oracle_comp
 
 section examples
 
-noncomputable theory
-
 -- This set of examples serves as sort of a "unit test" for the coercions above
-variables (spec spec' spec'' spec''' : oracle_spec)
+variables (α : Type) (spec spec' spec'' spec''' : oracle_spec)
   (coe_spec coe_spec' : oracle_spec)
   [coe_spec ⊂ₒ coe_spec']
 
@@ -245,7 +297,7 @@ example (oa : oracle_comp ((spec ++ spec') ++ (spec'' ++ coe_spec')) α) :
   oracle_comp (spec ++ spec' ++ spec'' ++ coe_spec') α := ↑oa
 
 /-- coercion makes it possible to mix computations on individual oracles -/
-example {spec : oracle_spec} : oracle_comp (unif_spec ++ spec) bool :=
+noncomputable example {spec : oracle_spec} : oracle_comp (unif_spec ++ spec) bool :=
 do { n ←$[0..3141], b ← coin, if n ≤ 1618 ∧ b = tt then return ff else coin }
 
 -- TODO!!!: does this work ever without deep recursion? probably not?
