src/computational_monads/simulation_semantics/oracle_append.lean
@@ -3,123 +3,53 @@ Copyright (c) 2022 Devon Tuma. All rights reserved.
 Released under Apache 2.0 license as described in the file LICENSE.
 Authors: Devon Tuma
 -/
-import computational_monads.coercions.instances
-import computational_monads.simulation_semantics.is_tracking
+import computational_monads.simulation_semantics.oracle_compose
 
 /-!
 # Appending Simulation Oracles
 
-This file defines an append operation `++ₛ` for simulation oracles,
+This file defines an append operation `++ₛₒ` for simulation oracles,
 creating a simulation oracle for a combined set of initial oracles.
 In particular, if simulation oracles `so` and `so'` have starting oracles given by
-`spec` and `spec'`, then `so ++ₛ so'` will have starting oracles `spec ++ spec'`.
+`spec` and `spec'`, then `so ++ₛₒ so'` will have starting oracles `spec ++ spec'`.
 
 The implementation just maintains a seperate state for each oracle,
 using pattern matching on queries to decide which `sim_oracle` to call.
+
+TODO: This has all been moved to the main file for now
 -/
 
-open oracle_comp oracle_spec
+-- open oracle_comp oracle_spec sum
 
-variables {spec spec' spec'' spec''' : oracle_spec} {α β γ : Type} {S S' : Type}
+-- variables {spec spec' spec'' spec''' : oracle_spec} {α β γ : Type} {S S' : Type}
 
-namespace sim_oracle
+-- namespace sim_oracle
 
-def oracle_append (so : sim_oracle spec spec'' S) (so' : sim_oracle spec' spec'' S') :
-  sim_oracle (spec ++ spec') spec'' (S × S') :=
-λ i, match i with
-| (sum.inl i) := λ ⟨t, s₁, s₂⟩, do {⟨u, s₁'⟩ ← so i (t, s₁), return (u, s₁', s₂)}
-| (sum.inr i) := λ ⟨t, s₁, s₂⟩, do {⟨u, s₂'⟩ ← so' i (t, s₂), return (u, s₁, s₂')}
-end
+-- def append (so : sim_oracle spec spec'' S) (so' : sim_oracle spec' spec'' S') :
+--   sim_oracle (spec ++ spec') spec'' (S × S') :=
+-- λ i, match i with
+-- | (inl i) := λ ⟨t, s₁, s₂⟩, do {⟨u, s₁'⟩ ← so i (t, s₁), return (u, s₁', s₂)}
+-- | (inr i) := λ ⟨t, s₁, s₂⟩, do {⟨u, s₂'⟩ ← so' i (t, s₂), return (u, s₁, s₂')}
+-- end
 
--- TODO: `++ₛₒ`??
-infixl ` ++ₛ `:65 := oracle_append
+-- infixl ` ++ₛₒ `:65 := append
 
-namespace oracle_append
+-- variables (so : sim_oracle spec spec'' S) (so' : sim_oracle spec' spec'' S')
 
-variables (so : sim_oracle spec spec'' S) (so' : sim_oracle spec' spec'' S')
-  (oa : oracle_comp (spec ++ spec') α) (ob : α → oracle_comp (spec ++ spec') β) (a : α)
-  (i : spec.ι) (i' : spec'.ι) (t : spec.domain i) (t' : spec'.domain i') (s : S × S')
-  (x : spec.domain i × S × S') (x' : spec'.domain i' × S × S')
+-- @[simp] lemma append_apply_inl (i : spec.ι) (x : spec.domain i × S × S') :
+--   (so ++ₛₒ so') (inl i) x = (λ z : spec.range i × S, (z.1, z.2, x.2.2)) <$> so i (x.1, x.2.1) :=
+-- begin
+--   rcases x with ⟨t, s₁, s₂⟩,
+--   refine congr_arg (λ ou, so i (t, s₁) >>= ou) (funext $ λ y, _),
+--   cases y, refl,
+-- end
 
-@[simp] lemma apply_inl_eq : (so ++ₛ so') (sum.inl i) x =
-  do {u_s' ← so i (x.1, x.2.1), return (u_s'.1, u_s'.2, x.2.2)} :=
-begin
-  cases x with t s, cases s with s₁ s₂,
-  refine congr_arg (λ ou, so i (t, s₁) >>= ou) (funext $ λ y, _),
-  cases y, refl,
-end
+-- @[simp] lemma append_apply_inr (i : spec'.ι) (x : spec'.domain i × S × S') :
+--   (so ++ₛₒ so') (inr i) x = (λ z : spec'.range i × S', (z.1, x.2.1, z.2)) <$> so' i (x.1, x.2.2) :=
+-- begin
+--   rcases x with ⟨t, s₁, s₂⟩,
+--   refine congr_arg (λ ou, so' i (t, s₂) >>= ou) (funext $ λ y, _),
+--   cases y, refl,
+-- end
 
-@[simp] lemma apply_inr_eq : (so ++ₛ so') (sum.inr i') x' =
-  do {u_s' ← so' i' (x'.1, x'.2.2), return (u_s'.1, x'.2.1, u_s'.2)} :=
-begin
-  cases x' with t s, cases s with s₁ s₂,
-  refine congr_arg (λ ou, so' i' (t, s₂) >>= ou) (funext $ λ y, _),
-  cases y, refl,
-end
-
-section support
-
-lemma support_apply_inl : ((so ++ₛ so') (sum.inl i) (t, s)).support =
-  {x | (x.1, x.2.1) ∈ (so i (t, s.1)).support ∧ x.2.2 = s.2} :=
-begin
-  ext x,
-  simp only [apply_inl_eq, support_bind, support_return, set.mem_Union,
-    set.mem_singleton_iff, exists_prop, prod.exists, set.mem_set_of_eq],
-  refine ⟨λ h, _, λ h, _⟩,
-  { obtain ⟨u, s', hu, hx⟩ := h,
-    simpa only [hx, eq_self_iff_true, and_true] using hu },
-  { refine ⟨x.1, x.2.1, _⟩,
-    simp only [← h.2, h.1, true_and, prod.mk.eta] }
-end
-
-lemma support_apply_inr : ((so ++ₛ so') (sum.inr i') (t', s)).support =
-  {x | (x.1, x.2.2) ∈ (so' i' (t', s.2)).support ∧ x.2.1 = s.1} :=
-begin
-  ext x,
-  simp only [apply_inr_eq, support_bind, support_return, set.mem_Union,
-    set.mem_singleton_iff, exists_prop, prod.exists, set.mem_set_of_eq],
-  refine ⟨λ h, _, λ h, _⟩,
-  { obtain ⟨u, s', hu, hx⟩ := h,
-    simpa only [hx, eq_self_iff_true, and_true] using hu },
-  { refine ⟨x.1, x.2.2, _⟩,
-    simp only [← h.2, h.1, true_and, prod.mk.eta] }
-end
-
-end support
-
-end oracle_append
-
-section coercions
-
--- TODO: there are more coercions that should be added here
--- It may be possible to move these into the instances file itself even
-
-variables variables (so : sim_oracle spec spec'' S) (so' : sim_oracle spec' spec'' S')
-
-@[simp] lemma simulate_coe_append_right (s : S × S') (oa : oracle_comp spec α) :
-  simulate (so ++ₛ so') ↑oa s = (λ (x : α × S), (x.1, x.2, s.2)) <$> simulate so oa s.1 :=
-begin
-  induction oa using oracle_comp.induction_on' with α a i t α oa hoa generalizing s,
-  { simp only [coe_sub_spec_return, simulate_return, map_pure, prod.mk.eta] },
-  { simp [hoa, bind_assoc] }
-end
-
-@[simp] lemma simulate'_coe_append_right (s : S × S') (oa : oracle_comp spec α) :
-  (simulate' (so ++ₛ so') ↑oa s) = simulate' so oa s.1 :=
-by simp [simulate'.def]
-
-@[simp] lemma simulate_coe_append_left (s : S × S') (oa : oracle_comp spec' α) :
-  simulate (so ++ₛ so') ↑oa s = (λ (x : α × S'), (x.1, s.1, x.2)) <$> simulate so' oa s.2 :=
-begin
-  induction oa using oracle_comp.induction_on' with α a i t α oa hoa generalizing s,
-  { simp only [coe_sub_spec_return, simulate_return, map_pure, prod.mk.eta] },
-  { simp [hoa, bind_assoc] }
-end
-
-@[simp] lemma simulate'_coe_append_left (s : S × S') (oa : oracle_comp spec' α) :
-  (simulate' (so ++ₛ so') ↑oa s) = simulate' so' oa s.2 :=
-by simp [simulate'.def]
-
-end coercions
-
-end sim_oracle
+-- end sim_oracle
